SumaIntToSumaNat 10%

CODIGO/SUMA/Transformations/SumaIntToSumaNat.dfy
@@ -22,18 +22,126 @@ function MultisetNatToInt(A:multiset<nat>) : (r:(multiset<int>))
         if (minInt == 0) then MultisetNatToInt(A-multiset{min}) else multiset{minInt} + MultisetNatToInt(A-multiset{min})
 }
 
-function SumaInt_to_SumaNat(A:multiset<int>, S:int) : (r:(multiset<nat>,nat))
-    requires forall e | e in A :: e > -10 && e < 10
-    requires S > -10 && S < 10
+ghost function GMultisetNegToPos(A:multiset<int>) : (r:(multiset<int>)) 
+requires forall e | e in A :: e < 0
+ensures forall e | e in r :: e > 0 && -e in A
+ensures forall e | -e in A :: e in r && r[e] == A[-e]
+//ensures forall e | e in A :: -e in r && r[-e] == A[e]//esto se queda colgado
+ensures |A| == |r|
+/*
 {
-    var SA:multiset<nat> := MultisetIntToNat(A);
-    var SS:nat := |A|*1000;
-    (SA,SS)
+    if A == multiset{} then multiset{}
+    else 
+        var m :| m in A; 
+        (multiset{-m} + GMultisetNegToPos(A-multiset{m}))
+}*/
+
+function FMultisetNegToPos(A:multiset<int>) : (r:(multiset<int>)) 
+requires forall e | e in A :: e < 0
+ensures r == GMultisetNegToPos(A)
+{
+    if A == multiset{} then multiset{}
+    else 
+        var min := minInt(A);
+        (multiset{-min} + FMultisetNegToPos(A-multiset{min}))
 }
 
+
+function FMultisetAbs(A:multiset<int>) : (r:(multiset<nat>)) 
+{
+    FPositiveElements(A) + FMultisetNegToPos(FNegativeElements(A))
+}
+
+ghost function GPositiveElements(A:multiset<int>) : (r:(multiset<int>)) 
+ensures r <= A 
+ensures forall e | e in A && e >= 0 :: e in r && r[e] == A[e]
+ensures forall e | e in r :: e >= 0 
+{  
+    if A == multiset{} then multiset{}
+    else 
+        var m :| m in A;
+        if m >= 0 then 
+            (multiset{m} + GPositiveElements(A - multiset{m}))
+        else
+            (GPositiveElements(A - multiset{m}))
+}
+
+function FPositiveElements(A:multiset<int>) : (r:(multiset<int>)) 
+ensures r == GPositiveElements(A)
+{  
+    if A == multiset{} then multiset{}
+    else 
+        var m := minInt(A);
+        if m >= 0 then 
+            (multiset{m} + FPositiveElements(A - multiset{m}))
+        else
+            (FPositiveElements(A - multiset{m}))
+}
+
+ghost function GNegativeElements(A:multiset<int>) : (r:(multiset<int>)) 
+ensures r <= A 
+ensures forall e | e in A && e < 0 :: r[e] == A[e]
+ensures forall e | e in r :: e < 0
+{  
+    if A == multiset{} then multiset{}
+    else 
+        var m :| m in A;
+        if m < 0 then 
+            (multiset{m} + GNegativeElements(A - multiset{m}))
+        else
+            (GNegativeElements(A - multiset{m}))
+} 
+
+function FNegativeElements(A:multiset<int>) : (r:(multiset<int>)) 
+ensures r == GNegativeElements(A)
+{  
+    if A == multiset{} then multiset{}
+    else 
+        var m := minInt(A);
+        if m < 0 then 
+            (multiset{m} + FNegativeElements(A - multiset{m}))
+        else
+            (FNegativeElements(A - multiset{m}))
+}
+
+
+
+function FMultisetAdd(A:multiset<int>, x:int) : (r:(multiset<nat>)) 
+requires x >=  FSumNat(FMultisetAbs(A))
+ensures forall e | e in A :: e + x !in A && e + x in r
+{  
+    if A == multiset{} then multiset{}
+    else 
+        var i := minInt(A);
+        assume i + x > 0;
+        (multiset{i+x} + FMultisetAdd(A - multiset{i},x))
+}
+
+function repeat(value:nat, amount:nat) : (r:(multiset<nat>)) 
+ensures r[value] == amount
+{  
+    if amount == 0 then multiset{}
+    else 
+        (multiset{value} + repeat(value,amount-1))
+}
+
+lemma SumAbsGtSum(A: multiset<int>)
+ensures FSumNat(FMultisetAbs(A)) >= FSumInt(A)
+
+
+function SumaInt_to_SumaNat(A:multiset<int>, S:int) : (r:(multiset<nat>,nat))
+{   
+    SumAbsGtSum(A);
+    var absSum := FSumNat(FMultisetAbs(A));
+    var SA:multiset<nat> := FMultisetAdd(A,absSum) + repeat(absSum, |A|);
+    var SS:int := S + |A|*absSum;
+
+    if (SS < 0) then (multiset{}, 5)
+    else (SA,SS)
+}
+
+
 lemma SumaInt_SumaNat(A:multiset<int>, S:int)
-    requires forall e | e in A :: e > -10 && e < 10
-    requires S > -10 && S < 10
     ensures var (SA, SS):= SumaInt_to_SumaNat(A, S);
           SumaInt(A,S) <==> SumaNat(SA, SS)
 { 
@@ -42,8 +150,6 @@ lemma SumaInt_SumaNat(A:multiset<int>, S:int)
 }
 
 lemma SumaInt_SumaNat1(A:multiset<int>, S:int)
-requires forall e | e in A :: e > -10 && e < 10
-    requires S > -10 && S < 10
     ensures var (SA, SS) := SumaInt_to_SumaNat(A, S);
           SumaInt(A,S) <== SumaNat(SA, SS)
 {   
@@ -58,8 +164,6 @@ requires forall e | e in A :: e > -10 && e < 10
 }
 
 lemma SumaInt_SumaNat2(A:multiset<int>, S:int)
-requires forall e | e in A :: e > -10 && e < 10
-    requires S > -10 && S < 10
     ensures var (SA, SS) := SumaInt_to_SumaNat(A, S);
           SumaInt(A,S) ==> SumaNat(SA,SS)
 {
